aarch64 refine: add bound for ppn in PageTablePTE
For ADT_C in CRefine, we need to know that the ppn in PageTablePTEs
cannot become too large, because we shift it left by pageBits (and we
need to show that this shift does not lose information).

Signed-off-by: Gerwin Klein <gerwin.klein@proofcraft.systems>

proof/refine/AARCH64/Invariants_H.thy
@@ -519,9 +519,17 @@ definition valid_mapping' :: "machine_word \<Rightarrow> vmpage_size \<Rightarro
 definition valid_vcpu' :: "vcpu \<Rightarrow> bool" where
   "valid_vcpu' v \<equiv> case vcpuTCBPtr v of None \<Rightarrow> True | Some vt \<Rightarrow> vt \<noteq> 0"
 
+(* This is a slight abuse of "canonical_address". What we really need to know for ADT_C in CRefine
+   is that the top pageBits bits of TablePTEs have a known value, because we shift left by pageBits.
+   What we actually know is that this is a physical address, so it is bound by the physical address
+   space size, which depending on config can be 40, 44, or 48. 48 happens to also be the bound for
+   the virtual address space, which canonical_address is for. This is good enough for our purposes. *)
+definition ppn_bounded :: "pte \<Rightarrow> bool" where
+  "ppn_bounded pte \<equiv> case pte of PageTablePTE ppn \<Rightarrow> canonical_address ppn | _ \<Rightarrow> True"
+
 definition valid_arch_obj' :: "arch_kernel_object \<Rightarrow> bool" where
   "valid_arch_obj' ako \<equiv> case ako of
-     KOPTE pte \<Rightarrow> True
+     KOPTE pte \<Rightarrow> ppn_bounded pte
    | KOVCPU vcpu \<Rightarrow> valid_vcpu' vcpu
    | _ \<Rightarrow> True"
 
